6.5 Type-checking example.

type_check.hs
@@ -1,0 +1,118 @@
+module Type_check where
+
+import qualified Prelude
+
+data Bool =
+   True
+ | False
+
+data Nat =
+   O
+ | S Nat
+
+type Sig a =
+  a
+  -- singleton inductive, whose constructor was exist
+  
+data Sumor a =
+   Inleft a
+ | Inright
+
+data Maybe a =
+   Unknown
+ | Found a
+
+data Exp =
+   Nat0 Nat
+ | Plus Exp Exp
+ | Bool0 Bool
+ | And Exp Exp
+
+data Type =
+   TNat
+ | TBool
+
+type_rect :: a1 -> a1 -> Type -> a1
+type_rect f f0 t =
+  case t of {
+   TNat -> f;
+   TBool -> f0}
+
+type_rec :: a1 -> a1 -> Type -> a1
+type_rec =
+  type_rect
+
+eq_type_dec :: Type -> Type -> Bool
+eq_type_dec t1 t2 =
+  type_rec (\t0 ->
+    case t0 of {
+     TNat -> True;
+     TBool -> False}) (\t0 ->
+    case t0 of {
+     TNat -> False;
+     TBool -> True}) t1 t2
+
+typeCheck :: Exp -> Maybe Type
+typeCheck e =
+  case e of {
+   Nat0 n -> Found TNat;
+   Plus e1 e2 ->
+    case typeCheck e1 of {
+     Unknown -> Unknown;
+     Found t1 ->
+      case typeCheck e2 of {
+       Unknown -> Unknown;
+       Found t2 ->
+        case eq_type_dec t1 TNat of {
+         True ->
+          case eq_type_dec t2 TNat of {
+           True -> Found TNat;
+           False -> Unknown};
+         False -> Unknown}}};
+   Bool0 b -> Found TBool;
+   And e1 e2 ->
+    case typeCheck e1 of {
+     Unknown -> Unknown;
+     Found t1 ->
+      case typeCheck e2 of {
+       Unknown -> Unknown;
+       Found t2 ->
+        case eq_type_dec t1 TBool of {
+         True ->
+          case eq_type_dec t2 TBool of {
+           True -> Found TBool;
+           False -> Unknown};
+         False -> Unknown}}}}
+
+typeCheck' :: Exp -> Sumor Type
+typeCheck' e =
+  case e of {
+   Nat0 n -> Inleft TNat;
+   Plus e1 e2 ->
+    case typeCheck' e1 of {
+     Inleft s ->
+      case typeCheck' e2 of {
+       Inleft s0 ->
+        case eq_type_dec s TNat of {
+         True ->
+          case eq_type_dec s0 TNat of {
+           True -> Inleft TNat;
+           False -> Inright};
+         False -> Inright};
+       Inright -> Inright};
+     Inright -> Inright};
+   Bool0 b -> Inleft TBool;
+   And e1 e2 ->
+    case typeCheck' e1 of {
+     Inleft s ->
+      case typeCheck' e2 of {
+       Inleft s0 ->
+        case eq_type_dec s TBool of {
+         True ->
+          case eq_type_dec s0 TBool of {
+           True -> Inleft TBool;
+           False -> Inright};
+         False -> Inright};
+       Inright -> Inright};
+     Inright -> Inright}}
+
